added subformula stuff, free/bound defn

ModelTheory.v
@@ -1,15 +1,22 @@
 Require Export Coq.Strings.String.
 
+(* Symbols *)
 Inductive var : Type :=
 | Var : string -> var.
+Inductive func : Type :=
+| Func : string -> func.
+Inductive const : Type :=
+| Const : string -> const.
 
+(* Terms *)
 (* FixMe: does this need a type param? *)
 Inductive term : Type :=
 | VarT   : var -> term
-| ConstT : string -> term
-| FuncT  : string -> (list term) -> term. (*FixMe: how to define arg list as non-empty? 
-                                            FuncT w/ empty arg list is same as a constant. *)
+| ConstT : const -> term
+| FuncT  : func -> (list term) -> term. (*FixMe: how to define arg list as non-empty? 
+                                          FuncT w/ empty arg list is same as a constant.*)
 
+(* Formulas *)
 (* FixMe: does this need a type param? *)
 Inductive formula : Type := 
 | Equals  : term -> term -> formula
@@ -18,14 +25,134 @@ Inductive formula : Type :=
 | Or      : formula -> formula -> formula
 | Forall  : var -> formula -> formula.
 
+(* Derived formulas *)
 Definition And (phi psi : formula) := Not (Or (Not phi) (Not psi)).
 Definition Impl (phi psi : formula) := Or (Not phi) psi.
 Definition Iff (phi psi : formula) := And (Impl phi psi) (Impl psi phi).
 Definition Exists (v : var) (phi : formula) := Not (Forall v (Not phi)).
 
+(* Subformulas *)
 Inductive subformula : formula -> formula -> Prop :=
 | SubIden   (psi phi : formula) : psi = phi -> subformula psi phi
 | SubNot    (psi phi : formula) : subformula (Not psi) phi -> subformula psi phi
-| SubOrL    (psi theta phi : formula) : subformula (Or psi theta) phi -> subformula psi phi
-| SubOrR    (psi theta phi : formula) : subformula (Or psi theta) phi -> subformula theta phi
+| SubOrL    (theta psi phi : formula) : subformula (Or theta psi) phi -> subformula theta phi
+| SubOrR    (theta psi phi : formula) : subformula (Or theta psi) phi -> subformula psi phi
 | SubForall (v : var) (psi phi : formula) : subformula (Forall v psi) phi -> subformula psi phi.
+
+Theorem SubAndL : forall (theta psi phi : formula), 
+  subformula (And theta psi) phi -> subformula theta phi.
+Proof.
+  intros.
+  unfold And in H.
+  apply SubNot in H.
+  apply SubOrL in H.
+  apply SubNot in H.
+  assumption.
+Qed.
+
+Theorem SubAndR : forall (theta psi phi : formula),
+  subformula (And theta psi) phi -> subformula psi phi.
+Proof.
+  intros.
+  unfold And in H.
+  apply SubNot in H.
+  apply SubOrR in H.
+  apply SubNot in H.
+  assumption.
+Qed.
+
+Theorem SubImplL : forall (theta psi phi : formula),
+  subformula (Impl theta psi) phi -> subformula theta phi.
+Proof.
+  intros.
+  unfold Impl in H.
+  apply SubOrL in H.
+  apply SubNot in H.
+  assumption.
+Qed.
+
+Theorem SubImplR : forall (theta psi phi : formula),
+  subformula (Impl theta psi) phi -> subformula psi phi.
+Proof.
+  intros.
+  unfold Impl in H.
+  apply SubOrR in H.
+  assumption.
+Qed.
+
+Theorem SubIffL : forall (theta psi phi : formula),
+  subformula (Iff theta psi) phi -> subformula theta phi.
+Proof.
+  intros.
+  unfold Iff in H.
+  apply SubAndL in H.
+  apply SubImplL in H.
+  assumption.
+Qed.
+
+Theorem SubIffR : forall (theta psi phi : formula),
+  subformula (Iff theta psi) phi -> subformula psi phi.
+Proof.
+  intros.
+  unfold Iff in H.
+  apply SubAndL in H.
+  apply SubImplR in H.
+  assumption.
+Qed.
+
+Theorem SubExists : forall (v : var) (psi phi : formula),
+  subformula (Exists v psi) phi -> subformula psi phi.
+Proof.
+  intros.
+  unfold Exists in H.
+  apply SubNot in H.
+  apply SubForall in H.
+  apply SubNot in H.
+  assumption.
+Qed.
+
+(* Bound and free variables *)
+
+Inductive bound: var -> formula -> Prop :=
+|BoundForall (v: var) (psi phi : formula) : subformula (Forall v psi) phi -> bound v phi.
+Fixpoint boundFun (v : var) (phi : formula) := match phi with
+| Equals _ _ => False
+| Relates _ _ => False
+| Not psi => boundFun v psi
+| Or theta psi => boundFun v theta \/ boundFun v psi
+| Forall v' phi => v = v' \/ boundFun v phi
+end.
+
+Definition free (v : var) (phi : formula) := not (bound v phi).
+Definition freeFun (v : var) (phi : formula) := not (boundFun v phi).
+
+Example boundEx: bound (Var "x") (Forall (Var "x") (Equals (VarT (Var "x")) (VarT (Var "x")))).
+Proof.
+  remember (Var "x") as v.
+  remember (Equals (VarT v) (VarT v)) as psi.
+  apply BoundForall with (psi := psi).
+  apply SubIden.
+  reflexivity.
+Qed.
+
+Example freeEx: free (Var "y") (Forall (Var "x") (Equals (VarT (Var "x")) (VarT (Var "x")))).
+Proof.
+  unfold free, not.
+  intros.
+  inversion H. subst.
+  inversion H0; subst.
+  - (*SubIden case *) 
+    discriminate H1.
+  - (*SubNot case *)
+    
+Admitted.
+
+Example freeFunEx : freeFun (Var "y") (Forall (Var "x") (Equals (VarT (Var "x")) (VarT (Var "x")))).
+Proof.
+  unfold freeFun, not.
+  intros.
+  unfold boundFun in H.
+  destruct H.
+  - discriminate H.
+  - assumption.
+Qed.
